src/Pipes/Prelude.v
@@ -1,9 +1,333 @@
 Require Import Hask.Prelude.
 Require Import Hask.Control.Monad.
+Require Import Hask.Control.Monad.Trans.Class.
 Require Import Hask.Data.Functor.Identity.
 Require Import P.Pipes.
 
 Generalizable All Variables.
+
+Section Bounded.
+
+Variable n : nat.
+Variable r : Type.
+Variable d : r.
+
+(*
+Instance Proxy_MonadTrans {a' a b' b} : MonadTrans (Proxy a' a b' b) :=
+{ lift := fun m _ _ A => @M a' a b' b m r A id
+}.
+
+Instance Proxy_MonadTransLaws {a' a b' b} : MonadTrans (Proxy a' a b' b) :=
+{ trans_law_1 := ;
+  trans_law_2 :=
+}.
+*)
+
+(*
+Definition repeatM `{Monad m} `(x : m a) : Producer' a m r :=
+  fun _ _ => lift x >~ cat (n:=n) (d:=d).
+
+replicateM :: Monad m => Int -> m a -> Producer' a m ()
+replicateM n m = lift m >~ take n
+*)
+
+Definition drain `{Monad m} {a} : Consumer' a m r :=
+  fun _ _ => forP (cat (n:=n) (d:=d)) discard.
+
+Definition map `{Monad m} `(f : a -> b) :
+  Pipe a b m r := forP (cat (n:=n) (d:=d)) (yield \o f).
+
+(*
+Definition mapM `{Monad m} (f : a -> m b) : Pipe a b m r :=
+  for cat $ fun a => do
+    b <- lift (f a) ;;
+    yield b.
+
+sequence :: Monad m => Pipe (m a) a m r
+sequence = mapM id
+*)
+
+Definition mapFoldable `{Monad m} `(f : a -> seq b) : Pipe a b m r :=
+  forP (cat (n:=n) (d:=d)) (fun x => each (f x) (x':=unit) (x:=a)).
+
+Definition filter `{Monad m} `(p : a -> bool) : Pipe a a m r :=
+  forP (cat (n:=n) (d:=d)) $ fun a => when (p a) (yield a).
+
+(*
+filterM :: Monad m => (a -> m Bool) -> Pipe a a m r
+filterM predicate = for cat $ \a -> do
+    b <- lift (predicate a)
+    when b (yield a)
+*)
+
+Definition take `{Monad m} (n' : nat) {a} : Pipe a a m unit :=
+  replicateM_ n' (await >>= yield).
+
+(*
+takeWhile :: Monad m => (a -> Bool) -> Pipe a a m ()
+takeWhile predicate = go
+  where
+    go = do
+        a <- await
+        if (predicate a)
+            then do
+                yield a
+                go
+            else return ()
+
+drop :: Monad m => Int -> Pipe a a m r
+drop n = do
+    replicateM_ n await
+    cat
+
+dropWhile :: Monad m => (a -> Bool) -> Pipe a a m r
+dropWhile predicate = go
+  where
+    go = do
+        a <- await
+        if (predicate a)
+            then go
+            else do
+                yield a
+                cat
+
+concat :: (Monad m, Foldable f) => Pipe (f a) a m r
+concat = for cat each
+
+elemIndices :: (Monad m, Eq a) => a -> Pipe a Int m r
+elemIndices a = findIndices (a ==)
+
+findIndices :: Monad m => (a -> Bool) -> Pipe a Int m r
+findIndices predicate = loop 0
+  where
+    loop n = do
+        a <- await
+        when (predicate a) (yield n)
+        loop $! n + 1
+
+scan :: Monad m => (x -> a -> x) -> x -> (x -> b) -> Pipe a b m r
+scan step begin done = loop begin
+  where
+    loop x = do
+        yield (done x)
+        a <- await
+        let x' = step x a
+        loop $! x'
+
+scanM :: Monad m => (x -> a -> m x) -> m x -> (x -> m b) -> Pipe a b m r
+scanM step begin done = do
+    x <- lift begin
+    loop x
+  where
+    loop x = do
+        b <- lift (done x)
+        yield b
+        a  <- await
+        x' <- lift (step x a)
+        loop $! x'
+
+chain :: Monad m => (a -> m ()) -> Pipe a a m r
+chain f = for cat $ \a -> do
+    lift (f a)
+    yield a
+
+fold :: Monad m => (x -> a -> x) -> x -> (x -> b) -> Producer a m () -> m b
+fold step begin done p0 = loop p0 begin
+  where
+    loop p x = case p of
+        Request v  _  -> closed v
+        Respond a  fu -> loop (fu ()) $! step x a
+        M          m  -> m >>= \p' -> loop p' x
+        Pure    _     -> return (done x)
+
+fold' :: Monad m => (x -> a -> x) -> x -> (x -> b) -> Producer a m r -> m (b, r)
+fold' step begin done p0 = loop p0 begin
+  where
+    loop p x = case p of
+        Request v  _  -> closed v
+        Respond a  fu -> loop (fu ()) $! step x a
+        M          m  -> m >>= \p' -> loop p' x
+        Pure    r     -> return (done x, r)
+
+foldM
+    :: Monad m
+    => (x -> a -> m x) -> m x -> (x -> m b) -> Producer a m () -> m b
+foldM step begin done p0 = do
+    x0 <- begin
+    loop p0 x0
+  where
+    loop p x = case p of
+        Request v  _  -> closed v
+        Respond a  fu -> do
+            x' <- step x a
+            loop (fu ()) $! x'
+        M          m  -> m >>= \p' -> loop p' x
+        Pure    _     -> done x
+
+foldM'
+    :: Monad m
+    => (x -> a -> m x) -> m x -> (x -> m b) -> Producer a m r -> m (b, r)
+foldM' step begin done p0 = do
+    x0 <- begin
+    loop p0 x0
+  where
+    loop p x = case p of
+        Request v  _  -> closed v
+        Respond a  fu -> do
+            x' <- step x a
+            loop (fu ()) $! x'
+        M          m  -> m >>= \p' -> loop p' x
+        Pure    r     -> do
+            b <- done x
+            return (b, r)
+
+all :: Monad m => (a -> Bool) -> Producer a m () -> m Bool
+all predicate p = null $ p >-> filter (\a -> not (predicate a))
+
+any :: Monad m => (a -> Bool) -> Producer a m () -> m Bool
+any predicate p = liftM not $ null (p >-> filter predicate)
+
+and :: Monad m => Producer Bool m () -> m Bool
+and = all id
+
+or :: Monad m => Producer Bool m () -> m Bool
+or = any id
+
+elem :: (Monad m, Eq a) => a -> Producer a m () -> m Bool
+elem a = any (a ==)
+
+notElem :: (Monad m, Eq a) => a -> Producer a m () -> m Bool
+notElem a = all (a /=)
+
+find :: Monad m => (a -> Bool) -> Producer a m () -> m (Maybe a)
+find predicate p = head (p >-> filter predicate)
+
+findIndex :: Monad m => (a -> Bool) -> Producer a m () -> m (Maybe Int)
+findIndex predicate p = head (p >-> findIndices predicate)
+
+head :: Monad m => Producer a m () -> m (Maybe a)
+head p = do
+    x <- next p
+    return $ case x of
+        Left   _     -> Nothing
+        Right (a, _) -> Just a
+
+index :: Monad m => Int -> Producer a m () -> m (Maybe a)
+index n p = head (p >-> drop n)
+
+last :: Monad m => Producer a m () -> m (Maybe a)
+last p0 = do
+    x <- next p0
+    case x of
+        Left   _      -> return Nothing
+        Right (a, p') -> loop a p'
+  where
+    loop a p = do
+        x <- next p
+        case x of
+            Left   _       -> return (Just a)
+            Right (a', p') -> loop a' p'
+
+length :: Monad m => Producer a m () -> m Int
+length = fold (\n _ -> n + 1) 0 id
+
+maximum :: (Monad m, Ord a) => Producer a m () -> m (Maybe a)
+maximum = fold step Nothing id
+  where
+    step x a = Just $ case x of
+        Nothing -> a
+        Just a' -> max a a'
+
+minimum :: (Monad m, Ord a) => Producer a m () -> m (Maybe a)
+minimum = fold step Nothing id
+  where
+    step x a = Just $ case x of
+        Nothing -> a
+        Just a' -> min a a'
+
+null :: Monad m => Producer a m () -> m Bool
+null p = do
+    x <- next p
+    return $ case x of
+        Left  _ -> True
+        Right _ -> False
+
+sum :: (Monad m, Num a) => Producer a m () -> m a
+sum = fold (+) 0 id
+
+product :: (Monad m, Num a) => Producer a m () -> m a
+product = fold ( * ) 1 id
+
+toList :: Producer a Identity () -> [a]
+toList = loop
+  where
+    loop p = case p of
+        Request v _  -> closed v
+        Respond a fu -> a:loop (fu ())
+        M         m  -> loop (runIdentity m)
+        Pure    _    -> []
+
+toListM :: Monad m => Producer a m () -> m [a]
+toListM = fold step begin done
+  where
+    step x a = x . (a:)
+    begin = id
+    done x = x []
+
+zip :: Monad m
+    => (Producer   a     m r)
+    -> (Producer      b  m r)
+    -> (Producer' (a, b) m r)
+zip = zipWith (,)
+
+zipWith :: Monad m
+    => (a -> b -> c)
+    -> (Producer  a m r)
+    -> (Producer  b m r)
+    -> (Producer' c m r)
+zipWith f = go
+  where
+    go p1 p2 = do
+        e1 <- lift $ next p1
+        case e1 of
+            Left r         -> return r
+            Right (a, p1') -> do
+                e2 <- lift $ next p2
+                case e2 of
+                    Left r         -> return r
+                    Right (b, p2') -> do
+                        yield (f a b)
+                        go p1' p2'
+
+tee :: Monad m => Consumer a m r -> Pipe a a m r
+tee p = evalStateP Nothing $ do
+    r <- up >\\ (hoist lift p //> dn)
+    ma <- lift get
+    case ma of
+        Nothing -> return ()
+        Just a  -> yield a
+    return r
+  where
+    up () = do
+        ma <- lift get
+        case ma of
+            Nothing -> return ()
+            Just a  -> yield a
+        a <- await
+        lift $ put (Just a)
+        return a
+    dn v = closed v
+
+generalize :: Monad m => Pipe a b m r -> x -> Proxy x a x b m r
+generalize p x0 = evalStateP x0 $ up >\\ hoist lift p //> dn
+  where
+    up () = do
+        x <- lift get
+        request x
+    dn a = do
+        x <- respond a
+        lift $ put x
+*)
 
 Fixpoint toListM `{Monad m} `(p : Producer a m unit) : m (seq a) :=
   match p with
@@ -12,15 +336,6 @@ Fixpoint toListM `{Monad m} `(p : Producer a m unit) : m (seq a) :=
   | M _     f t  => t >>= (toListM \o f)
   | Pure    _    => pure [::]
   end.
-
-Section Bounded.
-
-Variable n : nat.
-Variable r : Type.
-Variable d : r.
-
-Definition map `{Monad m} `(f : a -> b) :
-  Pipe a b m r := forP (cat (n:=n) (d:=d)) (yield \o f).
 
 End Bounded.
 
@@ -69,7 +384,8 @@ Proof.
     by congr (M _ _).
 Qed.
 
-Theorem toListM_each_id : forall a, toListM \o each =1 pure (a:=seq a).
+Theorem toListM_each_id : forall a,
+  toListM \o (fun xs => each (x':=False) (x:=unit) xs) =1 pure (a:=seq a).
 Proof. by move=> ?; elim=> //= [? ? ->]. Qed.
 
 End PipesLawsPrelude.
